Fix FutureCertify

src/prop/PFConsistent.v
@@ -20,6 +20,8 @@ Require Import Thread.
 Require Import PromiseConsistent.
 Require Import ReorderPromises.
 Require Import Mapping.
+Require Import Pred.
+Require Import Trace.
 
 Set Implicit Arguments.
 
@@ -29,6 +31,15 @@ Definition pf_consistent lang (e:Thread.t lang): Prop :=
   exists e2,
     (<<STEPS: rtc (tau (Thread.step true)) (Thread.mk _ (Thread.state e) (Thread.local e) (Thread.sc e) mem1) e2>>) /\
     (<<PROMISES: (Local.promises (Thread.local e2)) = Memory.bot>>).
+
+Definition pf_consistent_or_failure lang (e:Thread.t lang): Prop :=
+  forall mem1 (CAP: Memory.cap (Thread.memory e) mem1),
+  exists e2,
+    (<<STEPS: rtc (tau (Thread.step true)) (Thread.mk _ (Thread.state e) (Thread.local e) (Thread.sc e) mem1) e2>>) /\
+    ((exists e e3,
+         (<<STEP_FAILURE: Thread.step true e e2 e3 >>) /\
+         (<<EVENT_FAILURE: ThreadEvent.get_machine_event e = MachineEvent.failure>>)) \/
+     (<<PROMISES: (Local.promises (Thread.local e2)) = Memory.bot>>)).
 
 Lemma promise_step_is_racy
       lc1 mem1 loc from to msg lc2 mem2 kind
@@ -105,4 +116,125 @@ Proof.
     exploit rtc_union_step_nonpf_bot; [|eauto|].
     { eapply rtc_implies; [|eauto]. apply tau_union. }
     i. subst. esplits; eauto.
+Qed.
+
+Lemma consistent_pf_consistent_or_failure lang (e:Thread.t lang)
+      (WF: Local.wf (Thread.local e) (Thread.memory e))
+      (SC: Memory.closed_timemap (Thread.sc e) (Thread.memory e))
+      (MEM: Memory.closed (Thread.memory e))
+      (CONSISTENT: Thread.consistent e)
+  :
+    pf_consistent_or_failure e.
+Proof.
+  ii. exploit CONSISTENT; eauto. i. des.
+  - inv FAILURE. des.
+    hexploit tau_steps_pf_tau_steps; eauto; ss.
+    { inv STEP_FAILURE; inv STEP; ss.
+      inv LOCAL; ss; inv LOCAL0; ss.
+    }
+    { eapply Local.cap_wf; eauto. }
+    { eapply Memory.cap_closed_timemap; eauto. }
+    { eapply Memory.cap_closed; eauto. }
+    i. des.
+    exploit rtc_union_step_nonpf_failure.
+    { eapply rtc_implies; [|eauto]. apply tau_union. }
+    { eauto. }
+    { eauto. }
+    i. des.
+    esplits; eauto.
+  - exploit tau_steps_pf_tau_steps; eauto; ss.
+    { ii. rewrite PROMISES, Memory.bot_get in *.  congr. }
+    { eapply Local.cap_wf; eauto. }
+    { eapply Memory.cap_closed_timemap; eauto. }
+    { eapply Memory.cap_closed; eauto. }
+    i. des.
+    exploit rtc_union_step_nonpf_bot; [|eauto|].
+    { eapply rtc_implies; [|eauto]. apply tau_union. }
+    i. subst. esplits; eauto.
+Qed.
+
+Definition no_sc_consistent lang (e:Thread.t lang): Prop :=
+  forall mem1 (CAP: Memory.cap (Thread.memory e) mem1),
+  exists e2,
+    (<<STEPS: rtc (tau (@pred_step no_sc _)) (Thread.mk _ (Thread.state e) (Thread.local e) (Thread.sc e) mem1) e2>>) /\
+    __guard__((exists e e3,
+                  (<<STEP_FAILURE: Thread.step true e e2 e3 >>) /\
+                  (<<EVENT_FAILURE: ThreadEvent.get_machine_event e = MachineEvent.failure>>)) \/
+              (<<PROMISES: (Local.promises (Thread.local e2)) = Memory.bot>>)).
+
+Lemma consistent_no_sc_consistent lang (e:Thread.t lang)
+      (WF: Local.wf (Thread.local e) (Thread.memory e))
+      (SC: Memory.closed_timemap (Thread.sc e) (Thread.memory e))
+      (MEM: Memory.closed (Thread.memory e))
+      (CONSISTENT: Thread.consistent e)
+  :
+  no_sc_consistent e.
+Proof.
+  eapply consistent_pf_consistent_or_failure in CONSISTENT; eauto.
+  ii. exploit CONSISTENT; eauto. intros [e2 [STEPS FINAL]].
+  guardH FINAL. des.
+  eapply rtc_implies in STEPS; cycle 1.
+  { instantiate (1:= tau (@pred_step (fun _ => True)  _)).
+    i. inv H. econs; eauto. econs; eauto. econs; eauto.
+  }
+  eapply (@hold_or_not _ no_sc) in STEPS. des.
+  { esplits.
+    { eapply rtc_implies; [|eapply HOLD].
+      i. inv H. inv TSTEP. des. econs; eauto. econs; eauto.
+    }
+    { eauto. }
+  }
+  { esplits.
+    { eapply rtc_implies; [|eapply STEPS0].
+      i. inv H. inv TSTEP. des. econs; eauto. econs; eauto.
+    }
+    right. inv STEP. inv STEP0; inv STEP; ss. inv LOCAL; ss.
+    { inv LOCAL0. eapply PROMISES.
+      eapply NNPP in BREAKQ. destruct ordw; ss.
+    }
+    { inv LOCAL0. eapply PROMISES. auto. }
+  }
+Qed.
+
+Definition no_sc_trace_consistent lang (e:Thread.t lang): Prop :=
+  forall mem1 (CAP: Memory.cap (Thread.memory e) mem1),
+  exists tr0 tr1 e2,
+    (<<STEPS: Trace.steps (tr0++tr1) (Thread.mk _ (Thread.state e) (Thread.local e) (Thread.sc e) mem1) e2>>) /\
+    (<<NOSC: List.Forall (fun '(_, e) => no_sc e) (tr0++tr1)>>) /\
+    (<<SILENT: List.Forall (fun '(_, e) => ThreadEvent.get_machine_event e = MachineEvent.silent) tr0>>) /\
+    (<<TRACE: __guard__(((<<NIL: tr1 = []>>) /\ (<<PROMISES: Local.promises (Thread.local e2) = Memory.bot>>)) \/ (exists lc e, (<<EVENT: tr1 = [(lc, e)]>>) /\ (<<FAILURE: ThreadEvent.get_machine_event e = MachineEvent.failure>>)))>>).
+
+Lemma consistent_no_sc_trace_consistent lang (e:Thread.t lang)
+      (WF: Local.wf (Thread.local e) (Thread.memory e))
+      (SC: Memory.closed_timemap (Thread.sc e) (Thread.memory e))
+      (MEM: Memory.closed (Thread.memory e))
+      (CONSISTENT: Thread.consistent e)
+  :
+  no_sc_trace_consistent e.
+Proof.
+  eapply consistent_no_sc_consistent in CONSISTENT; eauto.
+  ii. exploit CONSISTENT; eauto. i. des.
+  eapply pred_steps_trace_steps in STEPS. des. red in x0. des.
+  { exists tr, [(Thread.local e2, e0)]. esplits; eauto.
+    { eapply Trace.plus_step_steps; eauto. }
+    { eapply List.Forall_app. split.
+      { eapply List.Forall_impl; eauto. i.
+        destruct a. ss. des. auto.
+      }
+      { econs; eauto. destruct e0; ss. }
+    }
+    { eapply List.Forall_impl; eauto. i.
+      destruct a. ss. des. auto.
+    }
+    { right. esplits; eauto. }
+  }
+  { eexists tr, []. rewrite List.app_nil_r. esplits; eauto.
+    { eapply List.Forall_impl; eauto. i.
+      destruct a. ss. des. auto.
+    }
+    { eapply List.Forall_impl; eauto. i.
+      destruct a. ss. des. auto.
+    }
+    { left. esplits; eauto. }
+  }
 Qed.
