src/ldrfpf/PFStep.v
@@ -236,23 +236,20 @@ Section LOCALPF.
     :
       pf_consistent th.
   Proof.
-  (*   eapply consistent_pf_consistent in CONSISTENT; eauto. *)
-  (*   exploit Memory.cap_exists; eauto. i. des. *)
-  (*   exploit Memory.max_concrete_timemap_exists. *)
-  (*   { eapply Memory.cap_closed; eauto. } i. des. *)
-  (*   exploit CONSISTENT; eauto. i. des. *)
-  (*   { eapply pf_promises_steps_trace in STEPS; eauto. des. *)
-  (*     exists tr. splits; auto. ii. *)
-  (*     exploit (@Memory.cap_inj (Thread.memory th) mem2 mem1); eauto. i. subst. *)
-  (*     esplits; eauto. *)
-  (*   } *)
-  (*   { eapply pf_promises_steps_trace in STEPS; eauto. des. *)
-  (*     exists tr. splits; auto. ii. *)
-  (*     exploit (@Memory.cap_inj (Thread.memory th) mem2 mem1); eauto. i. subst. *)
-  (*     esplits; eauto. *)
-  (*   } *)
-  (* Qed. *)
-  Admitted.
+    eapply consistent_pf_consistent_or_failure in CONSISTENT; eauto.
+    exploit Memory.cap_exists; eauto. i. des.
+    exploit CONSISTENT; eauto. i. des.
+    { eapply pf_promises_steps_trace in STEPS; eauto. des.
+      exists tr. splits; auto. ii.
+      exploit (@Memory.cap_inj (Thread.memory th) mem2 mem1); eauto. i. subst.
+      esplits; eauto.
+    }
+    { eapply pf_promises_steps_trace in STEPS; eauto. des.
+      exists tr. splits; auto. ii.
+      exploit (@Memory.cap_inj (Thread.memory th) mem2 mem1); eauto. i. subst.
+      esplits; eauto.
+    }
+  Qed.
 End LOCALPF.
 End PF.
 
